Add a candidate proof stating that concrete execution is a subset of abstract execution In the case of JmpZero, only the taken branch is explored abstractly, making it easier to reason about the concrete and abstract state
If both branches are explored abstractly, the concrete state would only correspond to one of them, since the pc is
part of the concrete and abstract states

dafny/abstract-interpreter/SimpleVerifierAnalysis.dfy
@@ -4,6 +4,7 @@ module SimpleVerifierAnalysis {
   import opened Lang
   import opened E = ConcreteEval
   import opened AbstractEval
+  import opened Ints
 
   datatype PathState = PathState(state: E.State, pc: int)
 
@@ -52,38 +53,75 @@ module SimpleVerifierAnalysis {
     Interval(0, 0)
   }
 
+  function init_conc_reg_state(r: Reg): u32 {
+    0
+  }
+
   function initial_abstract_state(stmt: Stmt): AbstractPathState {
     AbstractPathState(AbstractState(init_abs_reg_state), 0, [])
+  }
+
+  function initial_concrete_state(stmt: Stmt): PathState {
+    PathState(init_conc_reg_state, 0)
   }
 
   function push_stack(stack: seq<AbstractPathState>, new_state: AbstractPathState): seq<AbstractPathState> {
     stack + [new_state]
   }
 
-  function backtrack_stack(stack: seq<AbstractPathState>): seq<AbstractPathState>
-    ensures |backtrack_stack(stack)| > 0 ==> |backtrack_stack(stack)[|backtrack_stack(stack)| - 1].branch_pcs| > 0
+  function backtrack_stack(stack: seq<AbstractPathState>, concrete_stack: seq<PathState>): (seq<AbstractPathState>, seq<PathState>)
+    ensures |backtrack_stack(stack, concrete_stack).0| > 0 ==> |backtrack_stack(stack, concrete_stack).0[|backtrack_stack(stack, concrete_stack).0| - 1].branch_pcs| > 0
+    ensures |stack| == |concrete_stack| ==> |backtrack_stack(stack, concrete_stack).0| == |backtrack_stack(stack, concrete_stack).1|
+    ensures |stack| == |concrete_stack| && (forall j :: 0 <= j < |stack| ==> path_state_included(concrete_stack[j], stack[j]))
+            ==> (forall i :: 0 <= i < |backtrack_stack(stack, concrete_stack).1| ==> path_state_included(backtrack_stack(stack, concrete_stack).1[i], backtrack_stack(stack, concrete_stack).0[i]))
   {
-    if |stack| == 0 then
-      []
+    if |stack| == 0 || |concrete_stack| == 0 then
+      ([], [])
     else if |stack[|stack| - 1].branch_pcs| > 0 then
-      stack
+      (stack, concrete_stack)
     else
-      backtrack_stack(stack[..|stack| - 1])
+      backtrack_stack(stack[..|stack| - 1], concrete_stack[..|concrete_stack| - 1])
   }
 
-  method explore_abstract_paths(prog: Program, fuel: int)
+  predicate reg_included(c_v: u32, v: Val) {
+    v.lo <= c_v as int <= v.hi
+  }
+
+  predicate state_included(env: E.State, abs: AbstractState) {
+    forall r: Reg :: reg_included(env(r), abs.rs(r))
+  }
+
+  predicate path_state_included(path_state: PathState, abs_path_state: AbstractPathState) {
+    (path_state.pc == abs_path_state.pc) &&
+    (state_included(path_state.state, abs_path_state.state))
+  }
+
+  method explore_abstract_paths(prog: Program, fuel: int, init_conc_state: PathState, init_abstract_state: AbstractPathState)
     requires fuel >= 0
     requires |prog.stmts| > 0
+    requires path_state_included(init_conc_state, init_abstract_state)
   {
-    var stack : seq<AbstractPathState> := [initial_abstract_state(prog.stmts[0])];
+    var stack : seq<AbstractPathState> := [init_abstract_state];
     var fuel := fuel;
+    var concrete_stack : seq<PathState> := [init_conc_state];
+
+    assert (path_state_included(concrete_stack[0], stack[0]));
+    assert |concrete_stack| == |stack|;
 
     while fuel > 0 && |stack| > 0
+      invariant |concrete_stack| == |stack|
+      // Proving that the actual execution is a subset of the static path wrt all taken branches
+      invariant forall i :: 0 <= i < |stack| ==> path_state_included(concrete_stack[i], stack[i])
     {
-      // Pop topmost state from the stack
+      // Pop topmost state from the abstract path stack
       var cur_state := stack[|stack| - 1];
       var cur_pc := cur_state.pc;
       stack := stack[..|stack| - 1];
+
+      // Pop topmost state from the concrete path stack
+      var cur_conc_state := concrete_stack[|concrete_stack| - 1];
+      var cur_conc_pc := cur_conc_state.pc;
+      concrete_stack := concrete_stack[..|concrete_stack| - 1];
 
       if cur_pc < 0 || cur_pc > |prog.stmts| {
         // We should never encounter this
@@ -91,10 +129,15 @@ module SimpleVerifierAnalysis {
       }
 
       if cur_pc == |prog.stmts| {
+        // We hit the end of this concrete execution
+
+        // Commenting out backtracking code
         // We hit the end of the subroutine
         // Backtrack till an abstract state with |branch_pcs| > 0 and
         // explore one of those paths
-        stack := backtrack_stack(stack);
+        /*var s := backtrack_stack(stack, concrete_stack);
+        stack := s.0;
+        concrete_stack := s.1;
 
         if |stack| > 0 {
           var last_state := stack[|stack| - 1].state;
@@ -108,31 +151,69 @@ module SimpleVerifierAnalysis {
 
           var new_expl_state := AbstractPathState(last_state, new_pc, []);
           stack := push_stack(stack, new_expl_state);
+
+          var last_conc_state := concrete_stack[|concrete_stack| - 1].state;
+          var last_conc_pc := concrete_stack[|concrete_stack| - 1].pc;
+          concrete_stack := concrete_stack + [PathState(last_conc_state, new_pc)];
+
         }
         fuel := fuel - 1;
-        continue;
+        continue;*/
+        break;
       }
 
       // Continue exploring the path
       var cur_stmt := prog.stmts[cur_state.pc];
+      var conc_step := stmt_step(cur_conc_state.state, cur_stmt);
+
+      if conc_step.None? {
+        // Invalid Execution Path
+        break;
+      }
+
+
       match cur_stmt {
         case Assign(r, e) => {
+
           var v := AbstractEval.expr_eval(cur_state.state, e);
           var new_state := AbstractEval.update_state(cur_state.state, r, v);
           // We rewrite the branches array when this state is being popped off
           // Iff it is a branch instruction
           var new_abs_state := AbstractPathState(new_state, cur_pc + 1, []);
           stack := push_stack(stack, new_abs_state);
+
+          assert conc_step.v.1 == 1;
+          var new_conc_state := PathState(conc_step.v.0, cur_pc + conc_step.v.1);
+          concrete_stack := concrete_stack + [new_conc_state];
+
+          assert (path_state_included(new_conc_state, new_abs_state));
+          assert path_state_included(concrete_stack[|concrete_stack| - 1], stack[|stack| - 1]);
         }
 
         case JmpZero(r, offset) => {
           // Copied from AbstractEval.stmt_eval
           // imprecise analysis: we don't try to prove that this jump is or isn't taken
           var fall_through := AbstractPathState(cur_state.state, cur_pc + 1, []);
-          var jmp_state := AbstractPathState(cur_state.state, cur_pc, [cur_pc + offset as int]);
+          var jmp_targ := AbstractPathState(cur_state.state, cur_pc + offset as int, []);
+          var jmp_state := AbstractPathState(cur_state.state, cur_pc, []);
 
-          // Explore the fall_through case with the jmp offset pending in the branch_pcs seq
-          stack := push_stack(push_stack(stack, jmp_state), fall_through);
+          var jmp_conc_state := PathState(cur_conc_state.state, cur_pc);
+          var jmp_conc_targ := PathState(cur_conc_state.state, cur_pc + offset as int);
+          var conc_fall_through := PathState(cur_conc_state.state, cur_pc + 1);
+
+          assert (path_state_included(jmp_conc_targ, jmp_targ));
+          assert (path_state_included(conc_fall_through, fall_through));
+
+          // We are interested in only the actual branch that is taken
+          if conc_step.v.1 == offset as int {
+            // Explore the target branch
+            stack := push_stack(push_stack(stack, jmp_state), jmp_targ);
+            concrete_stack := concrete_stack + [jmp_conc_state] + [jmp_conc_targ];
+          } else {
+            stack := push_stack(push_stack(stack, jmp_state), fall_through);
+            concrete_stack := concrete_stack + [jmp_conc_state] + [conc_fall_through];
+          }
+          assert path_state_included(concrete_stack[|concrete_stack| - 1], stack[|stack| - 1]);
         }
       }
 
